\documentclass[twocolumn]{article}
\usepackage{amsmath}
\usepackage[pdfusetitle]{hyperref}
\usepackage[a4paper]{geometry}
\usepackage{microtype}
\usepackage{mathtools}
\usepackage{xfrac}

\geometry{margin=1in}

\title{STAT PHYS SCIENCE Final Cheat Sheet}
\author{Noppakorn Jiravaranun}
\date{\today}

\newcommand\Perm[2][^n]{\prescript{#1\mkern-2.5mu}{}P_{#2}}
\newcommand\Comb[2][^n]{\prescript{#1\mkern-0.5mu}{}C_{#2}}

\begin{document}
\maketitle

\section{Continuous Random Distribution}
\subsection{Uniform Distribution}
\begin{align*}
    f(x) = \frac{1}{b-a}, a \leq x \leq b
\end{align*}
\begin{align*}
    \mu = E(x) = \frac{(a+b)}{2}
\end{align*}
\begin{align*}
    \sigma^{2} = V(X) = \frac{(b-a)^{2}}{12}
\end{align*}
\subsection{Normal Distribution}
\begin{align*}
    E(X) = \mu
\end{align*}
\begin{align*}
    V(X) = \sigma^{2}
\end{align*}
\subsubsection{Standardizing a Normal Random Variable}
\begin{align*}
    Z = \frac{X-\mu}{\sigma}
\end{align*}
\begin{align*}
    P(X \leq x) = P(\frac{X-\mu}{\sigma} \leq \frac{x-\mu}{\sigma}) = P(Z < z)
\end{align*}
\subsection{Exponential Distribution}
\begin{align*}
    f(x) = \lambda e^{-\lambda x} \text{, for } 0 \leq x < \infty
\end{align*}
\begin{align*}
    \mu = E(X) = \frac{1}{\lambda} \text {  and  }
    \sigma^{2} = V(x) = \frac{1}{\lambda^{2}}
\end{align*}
\subsection{Gamma Distribution}
\begin{align*}
    \mu = E(X) = \frac{r}{\lambda} \text{  and  } \sigma^{2} = V(X) = \frac{r}{\lambda^{2}}
\end{align*}

\vfill\break

\section{Sampling Distribution}
\subsection{Probability Distribution of Mean $(\bar{X})$}
\subsubsection{Known Variance}
\begin{align*}
    Z = \frac{\bar{X}-\mu_{\bar{X}}} {\frac{\sigma}{\sqrt{n}}}
\end{align*}
\subsubsection{$n \geq 30$}
\begin{align*}
    Z = \frac{\bar{X}-\mu_{\bar{X}}}{\frac{s}{\sqrt{n}}}
\end{align*}
\subsubsection{Unknown Variance}
\begin{align*}
    T = \frac{X - \mu}{\frac{S}{\sqrt{n}}}
\end{align*}
has a $t$ distribution with $n-1$ degree of freedom.
\subsection{Probability Distribution of Difference of Mean $(\bar{X_{1}}-\bar{X_{2}})$}
\subsubsection{Central Limit Theorem $(n \geq 30)$}
\begin{align*}
    Z = \frac{\bar{X_{1}} - \bar{X_{2}} - (\mu_{1} - \mu_{2})}{\sqrt{\frac{\sigma_{1}^{2}}{n_{1}} + \frac{\sigma_{2}^{2}}{n_{2}}}}
\end{align*}
\subsubsection{$\sigma_{1}^{2} = \sigma_{2}^{2}$}
Random varaible T with degree of freedom $n_{1}+n_{2}-2$
\begin{align*}
    T = \frac{\bar{X_{1}} - \bar{X_{2}} - (\mu_{1} - \mu_{2})}{\sqrt{S_{p}^{2}(\frac{1}{n_{1}} + \frac{1}{n_{2}})}}
\end{align*}
\begin{align*}
    S^{2}_{p} = \frac{(n-1)s_{1}^{2}+(n-1)s_{2}^{2}}{n_{1} + n_{2} - 2}
\end{align*}
\subsubsection{$\sigma_{1}^{2} \neq \sigma_{2}^{2}$}
$t$ distribution with degree of freedom
\begin{align*}
    \nu = \frac{(\frac{s_{1}^{2}}{n_{1}} + \frac{s_{2}^{2}}{n_{2}})^{2}}{\frac{(s_{1}^{2}/n_{1})^{2}}{n_{1} - 1}\frac{}{} + \frac{(s_{2}^{2}/n_{2})^{2}}{n_{2} - 1}}
\end{align*}
\begin{align*}
    T = \frac{\bar{X_{1}} - \bar{X_{2}} - (\mu_{1} - \mu_{2})}{\sqrt{\frac{\sigma_{1}^{2}}{n_{1}} + \frac{\sigma_{2}^{2}}{n_{2}}}}
\end{align*}
\subsubsection{Dependent data between two groups}
\begin{align*}
    T(n-1) = \frac{\bar{D} - \mu_{D}}{\frac{\sigma_{D}}{\sqrt{n}}} \text{ with } \sigma_{D} \approx S_{D} = \sqrt{\frac{\sum_{j=1}^{n}D_{j}^{2} - nD^{2}}{n-1}}
\end{align*}
\subsection{Variance $(S^{2})$}
\begin{align*}
    \chi^{2}(n-1) = \frac{(n-1)S^{2}}{\sigma^{2}}
\end{align*}
\subsection{Variance Ratio $(\frac{S_{1}^{2}}{S_{2}^{2}})$}
\begin{align*}
    F = \frac{\sfrac{s_{1}^{2}}{\sigma_{1}^{2}}}{\sfrac{s_{2}^{2}}{\sigma_{2}^{2}}}
\end{align*}
\begin{align*}
    F(n_{1}-1, n_{2}-1) = \frac{S_{1}^2 / \sigma_{1}^{2}}{S_{2}^2 / \sigma_{2}^{2}}
\end{align*}
\subsection{Sample Ratio $(\hat{P})$}
\begin{align*}
    Z = \frac{\hat{P} - P}{\sqrt{\frac{P(1-P)}{n}}}
\end{align*}
\subsection{Between Sample Ratio $(\hat{P_{1}} - \hat{P_{2}})$}
\begin{align*}
    Z = \frac{\hat{P_{1}} - \hat{P_{2}} - (P_{1} - P_{2})}{\sqrt{\frac{P_{1}(1-P_{1})}{n_{1}} + \frac{P_{2}(1-P_{2})}{n_{2}}}}
\end{align*}

\vfill\break

\section{ANOVA}
\begin{align*}
    SST = \sum_{i=1}^{k}\sum_{j=1}^{n_{i}}y_{ij}^{2} - \frac{TT^2}{N}
\end{align*}
\begin{align*}
    SSB = \sum_{i=1}^{k}\frac{T_{i}^{2}}{n_{i}} - \frac{TT^2}{N}
\end{align*}
\begin{align*}
    SSW = SST - SSB
\end{align*}
\begin{align*}
    MSB = \frac{SSB}{k-1}
\end{align*}
\begin{align*}
    MSW = \frac{SSW}{N-k}
\end{align*}
\begin{align*}
    F = \frac{MSB}{MSE}
\end{align*}
\section{Regression}
\subsection{Correlation Coefficient}
\begin{align*}
    S_{xy} = \sum_{i=1}^{n}(x_{i}y_{i}) - \frac{\sum_{i=1}^{n}x_{i}\sum_{i=1}^{n}y_{i}}{n}
\end{align*}
\begin{align*}
    S_{xx} = \sum_{i=1}^{n}x_{i}^{2} - \frac{(\sum_{i=1}^{n}x_{i})^{2}}{n}
\end{align*}
\begin{align*}
    S_{xx} = \sum_{i=1}^{n}y_{i}^{2} - \frac{(\sum_{i=1}^{n}y_{i})^{2}}{n}
\end{align*}
\begin{align*}
    r = \frac{S_{xy}}{\sqrt{S_{xx}S_{yy}}}
\end{align*}
\subsection{Regression Analysis}
\begin{align*}
    \hat{y} = b_{0} + b_{1}x
\end{align*}
\begin{align*}
    b_{1} = \frac{S_{xy}}{S_{xx}}
\end{align*}
\begin{align*}
    b_{0} = \bar{y} - b_{1}\bar{x}
\end{align*}
\begin{align*}
    SEE = \sqrt{\frac{S_{yy} - b_{1} S_{xy}}{n-2}}
\end{align*}
\subsection{Coefficient of Determination}
\begin{align*}
    R^{2} = \frac{b_{1}S_{xy}}{S_{yy}}
\end{align*}
\end{document}